Fir/Wasm/Concrete.lean
@@ -13,3 +13,4 @@ import Fir.Wasm.Concrete.ConstructorHeapCorrectness
 import Fir.Wasm.Concrete.ProjectionCorrectness
 import Fir.Wasm.Concrete.TagMutationCorrectness
 import Fir.Wasm.Concrete.FieldMutationCorrectness
+import Fir.Wasm.Concrete.ScalarMutationCorrectness
